\documentclass{article}

\usepackage{pandekten}
\usepackage{dashrule}

\usepackage[compat=1.1.0]{tikz-feynman}

%workaround from link
\usetikzlibrary{external}
\immediate\write18{mkdir -p pgf-img}
\tikzexternalize[
  prefix=pgf-img/,
  system call={
    lualatex \tikzexternalcheckshellescape -halt-on-error -interaction=batchmode -jobname="\image" "\texsource" || rm "\image.pdf"
  },
]

\makeatletter
\newcommand*{\shifttext}[1]{%
  \settowidth{\@tempdima}{#1}%
  \hspace{-\@tempdima}#1%
}
\newcommand{\plabel}[1]{%
\shifttext{\textbf{#1}\quad}%
}
\newcommand{\prule}{%
\begin{center}%
\hdashrule[0.5ex]{.99\linewidth}{1pt}{1pt 2.5pt}%
\end{center}%
}

\makeatother

\newcommand{\minusbaseline}{\abovedisplayskip=0pt\abovedisplayshortskip=0pt~\vspace*{-\baselineskip}}%

\setlength{\parindent}{0pt}

\title{Assignment 2}
\author{Ze Chen}

\begin{document}

\maketitle

\plabel{1 (a)}%
\begingroup\minusbaseline
\begin{align*}
    &{\phantom{{}={}}} \langle \phi(p_1) \phi(p_2) \phi(p_3) \phi(p_4) \rangle_{\mathrm{c}} \\
    &= \feynmandiagram [inline=(c.base), horizontal=p1 to p2, small] {
        p1[particle=$p_1$] -- c[dot],
        p3[particle=$p_2$] -- c,
        p2[particle=$p_3$] -- c,
        p4[particle=$p_4$] -- c,
    }; + \sum_{\substack{(i,j,k,l) = \\ (1,2,3,4), \\ (1,3,2,4), \\ (1,4,2,3)}} \feynmandiagram [inline=(c2.base), horizontal=c1 to c2, small] {
        p1[particle=$p_i$] -- c1[dot],
        p3[particle=$p_j$] -- c1,
        p2[particle=$p_k$] -- c2[dot],
        p4[particle=$p_l$] -- c2,
        c1 --[half left] c2;
        c1 --[half right] c2;
    }; \\
    &= \delta^{(3)}(p_1 + p_2 + p_3 + p_4) \cdot \qty{-\lambda + \lambda^2 \sum_{\substack{(i,j,k,l) = \\ (1,2,3,4), \\ (1,3,2,4), \\ (1,4,2,3)}} \int \frac{\dd[3]{k}}{(2\pi)^3} \frac{1}{k^2 + m^2} \frac{1}{(k - p_i - p_j)^2 + m^2}}.
\end{align*}
\endgroup

\plabel{(b)}%
Setting all external momenta to zero we find
\begin{align*}
    &{\phantom{{}={}}} \langle \phi(p_1) \phi(p_2) \phi(p_3) \phi(p_4) \rangle_{\mathrm{c}} \\
    &= \delta^{(3)}(p_1 + p_2 + p_3 + p_4) \cdot \qty{-\lambda + 3 \lambda^2 \int \frac{\dd[3]{k}}{(2\pi)^3} \frac{1}{k^2 + m^2} \frac{1}{k^2 + m^2}} \\
    &= \delta^{(3)}(p_1 + p_2 + p_3 + p_4) \cdot \qty{-\lambda + \frac{3\lambda^2}{8\pi m}}.
\end{align*}
The case of $m\rightarrow 0$ suffers IR divergence.
The form of corrections will be $\delta^{(3)}(p_1 + p_2 + p_3 + p_4) \cdot \lambda^V / m^L$ where $V$ is the number of internal vertices and $L$ is the number of loops.

\prule

\plabel{2}%
The 1PI correction is given by
\begin{align*}
    -iM^2(p^2) &= \feynmandiagram [layered layout, inline=(p2.base), horizontal=p1 to p2, small] {
        p1[particle=$p$\vphantom{$Mg$}] -- c1[dot],
        c2[dot] -- p2[particle=$p$\vphantom{$Mg$}],
        c1 --[half left] c2;
        c1 --[half right] c2;
    }; + \feynmandiagram [layered layout, inline=(p2.base), horizontal=p1 to p2, small] {
        p1[particle=$p$\vphantom{$Mg$}] -- c1[crossed dot],
        c1 -- p2[particle=$p$\vphantom{$Mg$}],
    }; \\
    &= (-i\lambda)^2 \cdot \frac{1}{2} \int \frac{\dd[d]{k}}{(2\pi)^d} \frac{i}{k^2 - m^2} \frac{i}{(k - p)^2 - m^2} + i(p^2 \delta_Z - \delta_m) \\
    &= \frac{\lambda^2}{2} \cdot \frac{i}{(4\pi)^{3-\epsilon/2}} \Gamma\qty(\frac{\epsilon}{2}-1) \int_0^1 \dd{x} \qty(\frac{1}{\Delta})^{\epsilon/2-1} + i(p^2 \delta_Z - \delta_m) \\
    &= \frac{\lambda^2}{2} \cdot \frac{i}{(4\pi)^3} \int_0^1 \dd{x} \qty[-\frac{2\Delta}{\epsilon} + \Delta\qty(-1+\Delta-\log(4\pi)+\log\Delta) + \bigO(\epsilon)] \\
    &{\phantom{{}={}}} + i(p^2 \delta_Z - \delta_m),
\end{align*}
where $d = 6-\epsilon$, and
\[ \Delta = m^2 - x(1-x)p^2. \]
The renormalization conditions are
\begin{align*}
    -iM^2(p^2 = 0) &= \frac{\lambda^2}{2} \cdot \frac{i}{(4\pi)^3} \qty[-\frac{2m^2}{\epsilon} - m^2\qty(1-\gamma+\log(\frac{4\pi}{m^2}))] - i\delta_m = 0, \\
    -i\pdv{p^2} M^2(p^2 = 0)  &= \frac{\lambda^2}{2} \cdot \frac{i}{(4\pi)^3} \qty[\frac{1}{3\epsilon} - \frac{\gamma}{6} + \frac{1}{6}\log(\frac{4\pi}{m^2})] + i\delta_Z = 0.
\end{align*}
Therefore,
\begin{align*}
    \delta_m &= \frac{\lambda^2}{2} \cdot \frac{m^2}{(4\pi)^3} \qty[-\frac{2}{\epsilon} - \qty(1-\gamma+\log(\frac{4\pi}{m^2}))], \\
    \delta_Z &= -\frac{\lambda^2}{2} \cdot \frac{1}{(4\pi)^3} \qty[\frac{1}{3\epsilon} - \frac{\gamma}{6} + \frac{1}{6}\log(\frac{4\pi}{m^2})].
\end{align*}

The vertex correction is given by
\begin{align*}
    -i\mathcal{M}^{(3)}(p,q) &= \feynmandiagram [inline=(p1.base), horizontal=v1 to p1, small] {
        p1[particle=$q$\vphantom{$Mg$}] -- v1[dot],
        p2[particle=$p+q$] -- v2[dot],
        p3[particle=$p$] -- v3[dot],
        v1 -- v2,
        v1 -- v3,
        v2 -- v3,
    }; + \feynmandiagram [inline=(v.base), horizontal=v to p2, small] {
        p1 -- v[crossed dot],
        p2 -- v,
        p3 -- v,
    }; \\
    &= (-i\lambda)^3 \int \frac{\dd[d]{k}}{(2\pi)^d} \frac{i}{k^2 - m^2} \frac{i}{(k-p)^2 - m^2} \frac{i}{(k+q)^2 - m^2} - i\delta_\lambda \\
    &= -i \lambda^3 \cdot \frac{1}{(4\pi)^{3-\epsilon/2}} \int_0^1 \dd{y} \int_0^1 \dd{z} \Gamma\qty(\frac{\epsilon}{2}) \qty(\frac{1}{\Delta})^{\epsilon/2} - i\delta_\lambda  \\
    &= -i \lambda^3 \cdot \frac{1}{(4\pi)^3} \int_0^1 \dd{y} \int_0^1 \dd{z} \qty[\frac{2}{\epsilon} -\gamma + \log(4\pi) - \log\Delta + \bigO(\epsilon)] - i\delta_\lambda ,
\end{align*}
where $d = 6-\epsilon$, and
\[ \Delta = m^2 + p^2 y(y-1) - 2p\cdot q yz + q^2 z(z-1). \]
Setting $-i\mathcal{M}^{(3)}(p=0,q=0) = 0$ we find
\[ \delta_\lambda = -\lambda^3 \cdot \frac{1}{(4\pi)^3} \qty[\frac{2}{\epsilon} -\gamma + \log(\frac{4\pi}{m^2})]. \]

\prule

\plabel{3 (a)}%
Since
\[ m_p^2 - m^2 - M^2(m_p^2) = m_p^2 - m^2 - M^2(m^2) + \bigO(\lambda^4) = 0 \]
we find
\begin{align*}
    A\lambda^2 m^2 &= M^2(m^2) = -\frac{\lambda ^2 m^2 }{2304 \pi ^3}\left(-15 \log \left(\frac{4\pi }{m^2}\right)+3 \pi  \sqrt{3}-16\right).
\end{align*}

\plabel{(b)}%
Ignoring $\bigO(\lambda^4)$ contributions we find
\[ B\lambda^2 = \pdv{p^2}M^2(p^2=m^2) = \frac{\lambda ^2}{2304 \pi ^3}\left(3 \sqrt{3} \pi -17\right) . \]

\prule

\plabel{4}%
\textbf{Evaluation of the First Diagram}\quad
With
\[ \feynmandiagram [inline=(c2.base), horizontal=c1 to c2, small] {
    p1[particle=$p$\vphantom{$Mg$}] -- c1[dot],
    p2[particle=$q$\vphantom{$Mg$}] -- c1,
    c2[dot] -- p3,
    c2 -- p4,
    c1 --[half left] c2;
    c1 --[half right] c2;
}; = (-i\lambda)^2 \cdot i V\qty((p+q)^2) \]
we find
\begin{align*}
    &{\phantom{{}={}}}\feynmandiagram [layered layout, inline=(p2.base), horizontal=p1 to p2, small] {
        p1[particle=$p$\vphantom{$Mg$}] -- c1[dot],
        c2[dot] -- p2[particle=$p$\vphantom{$Mg$}],
        c1 --[half left] c2;
        c1 --[half right] c2;
        c1 -- c2,
    }; \\
    &= \frac{1}{3} \int \frac{\dd[d]{q}}{(2\pi)^d} \frac{i}{q^2 - m^2} (-i\lambda)^2 iV\qty((p+q)^2) \\
    &= \frac{1}{3}\qty(-\frac{1}{2}) \int \frac{\dd[d]{q}}{(2\pi)^d} \frac{-1}{q^2 - m^2} (-i\lambda)^2 \int_0^1 \dd{x} \frac{\Gamma(2-d/2)}{(4\pi)^{d/2}} \cdot \frac{1}{\qty(m^2 - x(1-x)(p+q)^2)^{2-d/2}} \\
    &= \frac{1}{6}\lambda^2 \frac{\Gamma(3-d/2)}{(4\pi)^{d/2}} \int \frac{\dd[d]{q}}{(2\pi)^d} \int_0^1 \dd{x} \int_0^1 \dd{w}\\
    &\omit$\displaystyle\hfill \frac{w^{1-d/2}}{\qty(w(m^2 - x(1-x)(p+q)^2) - (1-w)(q^2 - m^2))^{3-d/2}}$ \\
    &= \frac{i \lambda^2}{6} \frac{\Gamma(3-d)}{(4\pi)^d} \int_0^1 \dd{x} \int_0^1 \dd{w} \frac{1}{\qty(1-w+wx(1-x))^{d/2}} w^{1-d/2} \qty(\frac{1}{\Delta})^{3-d}
\end{align*}
where
\[ \Delta = m^2 - \frac{w(1-w)x(1-x)}{1-w+wx(1-x)}p^2. \]
For $d = 4-\epsilon$,
\begin{align*}
    &{\phantom{{}={}}}\feynmandiagram [layered layout, inline=(p2.base), horizontal=p1 to p2, small] {
        p1[particle=$p$\vphantom{$Mg$}] -- c1[dot],
        c2[dot] -- p2[particle=$p$\vphantom{$Mg$}],
        c1 --[half left] c2;
        c1 --[half right] c2;
        c1 -- c2,
    }; \\
    &= \frac{i\lambda^2}{6}\frac{1}{(4\pi)^4} p^2 \int_0^1 \dd{x} \int_0^1 \dd{w} \qty(-\frac{1}{\epsilon} + \bigO(1))\qty(1-\epsilon \log p^2) f(x,w) \qty(1 - \epsilon \log g(x,w))
\end{align*}
where
\[ f(x,w) = -\frac{(1-w)x(1-x)}{\qty(1-w+wx(1-x))^3} \]
while $g(x,w)$ is not important.
Keeping only terms involving $\epsilon^{-1}$ and $\log p^2$ we find
\begin{align*}
    &{\phantom{{}={}}}\feynmandiagram [layered layout, inline=(p2.base), horizontal=p1 to p2, small] {
        p1[particle=$p$\vphantom{$Mg$}] -- c1[dot],
        c2[dot] -- p2[particle=$p$\vphantom{$Mg$}],
        c1 --[half left] c2;
        c1 --[half right] c2;
        c1 -- c2,
    }; \\
    &= \frac{i\lambda^2}{6}\frac{1}{(4\pi)^4} p^2 \qty(-\frac{1}{\epsilon} + \log p^2 + \cdots)\int_0^1 \dd{x} \int_0^1 \dd{w} f(x,w) \\
    &= \frac{i\lambda^2}{12}\frac{1}{(4\pi)^4} p^2 \qty(-\frac{1}{\epsilon} + \log p^2 + \cdots).
\end{align*}

\textbf{The Second Diagram Vanishes}\quad
\begin{align*}
    \feynmandiagram [layered layout, inline=(p2.base), horizontal=p1 to p2, small] {
        p1[particle=$p$\vphantom{$Mg$}] -- c1[crossed dot],
        c1 -- p2[particle=$p$\vphantom{$Mg$}],
        c1 --[out=135,in=45,loop,min distance=4em] c1,
    }; &= -i\delta_\lambda \int \frac{\dd[d]{p}}{(2\pi)^d} \frac{i}{p^2 - m^2} = m^{d-2} \cdot \bigO(m^\epsilon) \rightarrow 0
\end{align*}
as $m\rightarrow 0$.

\end{document}
